separating the inference from checker

pulse/examples/dsls/mini_steel/Pulse.Checker.fst
@@ -107,140 +107,6 @@ let check_abs
          tt |)
     | _ -> T.fail "bad hint"
 
-
-let rec infer_gen_uvars (t_head:term) : T.Tac (list term & comp) =
-  match t_head with
-  | Tm_Arrow {binder_ty=t} (Some Implicit) c_rest -> (
-    let uv = gen_uvar t in
-    let c_rest = open_comp_with c_rest uv in
-    match c_rest with
-    | C_ST c -> [uv], c_rest
-    | C_Tot t ->
-      let uv_rest, comp_typ = infer_gen_uvars t in
-      uv::uv_rest, comp_typ
-  )
-  | _ ->
-   T.fail (FStar.Printf.sprintf "infer_gen_uvars: unexpected t_head: %s"
-                                  (P.term_to_string t_head))
-
-let rec infer_check_valid_solution (t1 t2:term) (uv_sols:list (term & term))
-  : T.Tac (list (term & term)) =
-
-  match uv_sols with
-  | [] -> [t1, t2]
-  | (t1', t2')::tl ->
-    if t1 = t1'
-    then if t2 = t2' then uv_sols
-         else T.fail "infer_check_valid_solution failed"
-    else (t1', t2')::(infer_check_valid_solution t1 t2 tl)
-
-let rec infer_match_typ (t1 t2:term) (uv_sols:list (term & term))
-  : T.Tac (list (term & term)) =
-
-  match t1, t2 with
-  | Tm_UVar n, _ ->
-    infer_check_valid_solution t1 t2 uv_sols
-  | _, Tm_UVar _ -> T.fail "infer_match_typ: t2 is a uvar"
-
-  | Tm_PureApp head1 arg_qual1 arg1, Tm_PureApp head2 arg_qual2 arg2 ->
-    if arg_qual1 = arg_qual2
-    then let uv_sols = infer_match_typ head1 head2 uv_sols in
-         infer_match_typ arg1 arg2 uv_sols
-    else uv_sols
-
-  | _, _ -> uv_sols
-
-let rec infer_atomic_vprop_has_uvar (t:term) : bool =
-  match t with
-  | Tm_UVar _ -> true
-  | Tm_PureApp head _ arg ->
-    infer_atomic_vprop_has_uvar head || infer_atomic_vprop_has_uvar arg
-  | Tm_Emp -> false
-  | _ -> false
-
-let rec infer_atomic_vprops_may_match (t1:term) (t2:pure_term) : bool =
-  match t1, t2 with
-  | Tm_UVar _, _ -> true
-  | Tm_PureApp head1 q1 arg1, Tm_PureApp head2 q2 arg2 ->
-    infer_atomic_vprops_may_match head1 head2 &&
-    q1 = q2 &&
-    infer_atomic_vprops_may_match arg1 arg2
-  | _, _ -> t1 = t2
-
-let infer_one_atomic_vprop (t:pure_term) (ctxt:list pure_term) (uv_sols:list (term & term))
-  : T.Tac (list (term & term)) =
-
-  if infer_atomic_vprop_has_uvar t
-  then
-    let matching_ctxt = List.Tot.filter (fun ctxt_vp -> infer_atomic_vprops_may_match t ctxt_vp) ctxt in
-    // T.print (FStar.Printf.sprintf "infer_one_atomic_vprop %s, found %d matching candidates\n"
-    //            (P.term_to_string t)
-    //            (List.Tot.length matching_ctxt));
-    if List.Tot.length matching_ctxt = 1
-    then
-      // let _ = T.print (FStar.Printf.sprintf "infer_one_atomic_vprop: matching %s and %s with %d exisiting solutions\n"
-      //                    (P.term_to_string t)
-      //                    (P.term_to_string (List.Tot.hd matching_ctxt))
-      //                    (List.Tot.length uv_sols)) in 
-      let uv_sols = infer_match_typ t (List.Tot.hd matching_ctxt) uv_sols in
-      // T.print (FStar.Printf.sprintf "post matching, uv_sols has %d solutions\n"
-      //            (List.Tot.length uv_sols));
-      uv_sols
-    else uv_sols
-  else uv_sols
-
-let rec infer_build_head (head:term) (uvs:list term) (uv_sols:list (term & term))
-  : T.Tac term
-  = match uvs with
-    | [] -> head
-    | hd::tl ->
-      let ropt = List.Tot.find (fun (t1, _) -> t1 = hd) uv_sols in
-      match ropt with
-      | None -> T.fail "inference failed in building head"
-      | Some (_, t2) ->
-        match tl with
-        | [] -> Tm_STApp head (Some Implicit) t2
-        | _ ->
-          let app_node = Tm_PureApp head (Some Implicit) t2 in
-          infer_build_head app_node tl uv_sols
-
-let infer
-  (head:term)
-  (t_head:term)
-  (ctxt_pre:term)
-  
-  : T.Tac term =
-
-  let uvs, pre =
-    let uvs, comp = infer_gen_uvars t_head in
-    match comp with
-    | C_ST st_comp -> uvs, st_comp.pre
-    | _ -> T.fail "infer:unexpected comp type"
-  in
-
-  if List.Tot.length uvs = 0
-  then head
-  else begin
-    // T.print (FStar.Printf.sprintf "infer: generated %d uvars, ctx: %s, st_comp.pre: %s\n"
-    //            (List.Tot.length uvs)
-    //            (P.term_to_string ctxt_pre)
-    //            (P.term_to_string pre));
-
-    let uv_sols = [] in
-    
-    assume (is_pure_term pre);
-    let pre_list = vprop_as_list pre in
-
-    assume (is_pure_term ctxt_pre);
-    let ctxt_pre_list = vprop_as_list ctxt_pre in
-
-    let uv_sols = T.fold_left (fun uv_sols st_pre_vprop ->
-      infer_one_atomic_vprop st_pre_vprop ctxt_pre_list uv_sols) uv_sols pre_list in
-
-    let head = infer_build_head head uvs uv_sols in
-    head
-  end
-
 #push-options "--query_stats --fuel 2 --ifuel 1 --z3rlimit_factor 4"
 #push-options "--print_implicits --print_universes --print_full_names"
 let rec check' : bool -> check_t =
@@ -306,7 +172,7 @@ let rec check' : bool -> check_t =
           let head = Tm_PureApp head qual arg in
           let C_Tot ty_head = open_comp_with comp_typ arg in
           //Some implicits to follow
-          let t = infer head ty_head pre in
+          let t = Pulse.Checker.Inference.infer head ty_head pre in
           check' false f g t pre pre_typing post_hint
 
         | _ ->
