pulse/examples/dsls/mini_steel/Pulse.Checker.Inference.fst
@@ -1,0 +1,145 @@
+module Pulse.Checker.Inference
+
+module L = FStar.List.Tot
+module T = FStar.Tactics
+open FStar.List.Tot
+open Pulse.Syntax
+open Pulse.Elaborate.Pure
+open Pulse.Typing
+open Pulse.Checker.Framing
+module P = Pulse.Syntax.Printer
+
+module RT = Refl.Typing
+
+let rec gen_uvars (t_head:term) : T.Tac (list term & comp) =
+  match t_head with
+  | Tm_Arrow {binder_ty=t} (Some Implicit) c_rest -> (
+    let uv = gen_uvar t in
+    let c_rest = open_comp_with c_rest uv in
+    match c_rest with
+    | C_ST c -> [uv], c_rest
+    | C_Tot t ->
+      let uv_rest, comp_typ = gen_uvars t in
+      uv::uv_rest, comp_typ
+  )
+  | _ ->
+   T.fail (FStar.Printf.sprintf "gen_uvars: unexpected t_head: %s"
+                                  (P.term_to_string t_head))
+
+let rec check_valid_solution (t1 t2:term) (uv_sols:list (term & term))
+  : T.Tac (list (term & term)) =
+
+  match uv_sols with
+  | [] -> [t1, t2]
+  | (t1', t2')::tl ->
+    if t1 = t1'
+    then if t2 = t2' then uv_sols
+         else T.fail "check_valid_solution failed"
+    else (t1', t2')::(check_valid_solution t1 t2 tl)
+
+let rec match_typ (t1 t2:term) (uv_sols:list (term & term))
+  : T.Tac (list (term & term)) =
+
+  match t1, t2 with
+  | Tm_UVar n, _ ->
+    check_valid_solution t1 t2 uv_sols
+  | _, Tm_UVar _ -> T.fail "match_typ: t2 is a uvar"
+
+  | Tm_PureApp head1 arg_qual1 arg1, Tm_PureApp head2 arg_qual2 arg2 ->
+    if arg_qual1 = arg_qual2
+    then let uv_sols = match_typ head1 head2 uv_sols in
+         match_typ arg1 arg2 uv_sols
+    else uv_sols
+
+  | _, _ -> uv_sols
+
+let rec atomic_vprop_has_uvar (t:term) : bool =
+  match t with
+  | Tm_UVar _ -> true
+  | Tm_PureApp head _ arg ->
+    atomic_vprop_has_uvar head || atomic_vprop_has_uvar arg
+  | Tm_Emp -> false
+  | _ -> false
+
+let rec atomic_vprops_may_match (t1:term) (t2:pure_term) : bool =
+  match t1, t2 with
+  | Tm_UVar _, _ -> true
+  | Tm_PureApp head1 q1 arg1, Tm_PureApp head2 q2 arg2 ->
+    atomic_vprops_may_match head1 head2 &&
+    q1 = q2 &&
+    atomic_vprops_may_match arg1 arg2
+  | _, _ -> t1 = t2
+
+let infer_one_atomic_vprop (t:pure_term) (ctxt:list pure_term) (uv_sols:list (term & term))
+  : T.Tac (list (term & term)) =
+
+  if atomic_vprop_has_uvar t
+  then
+    let matching_ctxt = List.Tot.filter (fun ctxt_vp -> atomic_vprops_may_match t ctxt_vp) ctxt in
+    // T.print (FStar.Printf.sprintf "infer_one_atomic_vprop %s, found %d matching candidates\n"
+    //            (P.term_to_string t)
+    //            (List.Tot.length matching_ctxt));
+    if List.Tot.length matching_ctxt = 1
+    then
+      // let _ = T.print (FStar.Printf.sprintf "infer_one_atomic_vprop: matching %s and %s with %d exisiting solutions\n"
+      //                    (P.term_to_string t)
+      //                    (P.term_to_string (List.Tot.hd matching_ctxt))
+      //                    (List.Tot.length uv_sols)) in 
+      let uv_sols = match_typ t (List.Tot.hd matching_ctxt) uv_sols in
+      // T.print (FStar.Printf.sprintf "post matching, uv_sols has %d solutions\n"
+      //            (List.Tot.length uv_sols));
+      uv_sols
+    else uv_sols
+  else uv_sols
+
+let rec rebuild_head (head:term) (uvs:list term) (uv_sols:list (term & term))
+  : T.Tac term
+  = match uvs with
+    | [] -> head
+    | hd::tl ->
+      let ropt = List.Tot.find (fun (t1, _) -> t1 = hd) uv_sols in
+      match ropt with
+      | None -> T.fail "inference failed in building head"
+      | Some (_, t2) ->
+        match tl with
+        | [] -> Tm_STApp head (Some Implicit) t2
+        | _ ->
+          let app_node = Tm_PureApp head (Some Implicit) t2 in
+          rebuild_head app_node tl uv_sols
+
+let infer
+  (head:term)
+  (t_head:term)
+  (ctxt_pre:term)
+  
+  : T.Tac term =
+
+  let uvs, pre =
+    let uvs, comp = gen_uvars t_head in
+    match comp with
+    | C_ST st_comp -> uvs, st_comp.pre
+    | _ -> T.fail "infer:unexpected comp type"
+  in
+
+  if List.Tot.length uvs = 0
+  then head
+  else begin
+    // T.print (FStar.Printf.sprintf "infer: generated %d uvars, ctx: %s, st_comp.pre: %s\n"
+    //            (List.Tot.length uvs)
+    //            (P.term_to_string ctxt_pre)
+    //            (P.term_to_string pre));
+
+    let uv_sols = [] in
+    
+    assume (is_pure_term pre);
+    let pre_list = vprop_as_list pre in
+
+    assume (is_pure_term ctxt_pre);
+    let ctxt_pre_list = vprop_as_list ctxt_pre in
+
+    let uv_sols = T.fold_left (fun uv_sols st_pre_vprop ->
+      infer_one_atomic_vprop st_pre_vprop ctxt_pre_list uv_sols) uv_sols pre_list in
+
+    let head = rebuild_head head uvs uv_sols in
+    head
+  end
