pulse/examples/dsls/mini_steel/Pulse.Checker.Inference.fsti
@@ -1,0 +1,8 @@
+module Pulse.Checker.Inference
+
+open Pulse.Syntax
+
+module T = FStar.Tactics
+
+val infer (head:term) (t_head:term) (ctxt_pre:term)
+  : T.Tac term
